# 2023-09-13

- Today we worked on the SOMERUNS Example 1e, which describes an existential
hybrid program which aims to prove that there exists a run of A and B that
proves some post condition

- ## the proof progress is here (collapsed)

    ```KeYmaera
    iterated('R=="<{{x'=v,v'=a&x<=bf()}++{?x=bf();vi:=v;}{x'=v,v'=-vi^2/(2*(E()-bf()))&x>=bf()}}*>(x=E()&v=0)");
    iterated('R=="x=E()&v=0|<{x'=v,v'=a&x<=bf()}++{?x=bf();vi:=v;}{x'=v,v'=-vi^2/(2*(E()-bf()))&x>=bf()}>#<{{x'=v,v'=a&x<=bf()}++{?x=bf();vi:=v;}{x'=v,v'=-vi^2/(2*(E()-bf()))&x>=bf()}}*>(x=E()&v=0)#");
    orR('R=="x=E()&v=0|<{x'=v,v'=a&x<=bf()}++{?x=bf();vi:=v;}{x'=v,v'=-vi^2/(2*(E()-bf()))&x>=bf()}>(x=E()&v=0|<{x'=v,v'=a&x<=bf()}++{?x=bf();vi:=v;}{x'=v,v'=-vi^2/(2*(E()-bf()))&x>=bf()}><{{x'=v,v'=a&x<=bf()}++{?x=bf();vi:=v;}{x'=v,v'=-vi^2/(2*(E()-bf()))&x>=bf()}}*>(x=E()&v=0))");
    iterated('R=="<{x'=v,v'=a&x<=bf()}++{?x=bf();vi:=v;}{x'=v,v'=-vi^2/(2*(E()-bf()))&x>=bf()}>(x=E()&v=0|<{x'=v,v'=a&x<=bf()}++{?x=bf();vi:=v;}{x'=v,v'=-vi^2/(2*(E()-bf()))&x>=bf()}>#<{{x'=v,v'=a&x<=bf()}++{?x=bf();vi:=v;}{x'=v,v'=-vi^2/(2*(E()-bf()))&x>=bf()}}*>(x=E()&v=0)#)");
    diamondOr('R=="<{x'=v,v'=a&x<=bf()}++{?x=bf();vi:=v;}{x'=v,v'=-vi^2/(2*(E()-bf()))&x>=bf()}>(x=E()&v=0|#<{x'=v,v'=a&x<=bf()}++{?x=bf();vi:=v;}{x'=v,v'=-vi^2/(2*(E()-bf()))&x>=bf()}>(x=E()&v=0|<{x'=v,v'=a&x<=bf()}++{?x=bf();vi:=v;}{x'=v,v'=-vi^2/(2*(E()-bf()))&x>=bf()}><{{x'=v,v'=a&x<=bf()}++{?x=bf();vi:=v;}{x'=v,v'=-vi^2/(2*(E()-bf()))&x>=bf()}}*>(x=E()&v=0))#)");
    diamondOr('R=="<{x'=v,v'=a&x<=bf()}++{?x=bf();vi:=v;}{x'=v,v'=-vi^2/(2*(E()-bf()))&x>=bf()}>(x=E()&v=0|<{x'=v,v'=a&x<=bf()}++{?x=bf();vi:=v;}{x'=v,v'=-vi^2/(2*(E()-bf()))&x>=bf()}>(x=E()&v=0)|<{x'=v,v'=a&x<=bf()}++{?x=bf();vi:=v;}{x'=v,v'=-vi^2/(2*(E()-bf()))&x>=bf()}><{x'=v,v'=a&x<=bf()}++{?x=bf();vi:=v;}{x'=v,v'=-vi^2/(2*(E()-bf()))&x>=bf()}><{{x'=v,v'=a&x<=bf()}++{?x=bf();vi:=v;}{x'=v,v'=-vi^2/(2*(E()-bf()))&x>=bf()}}*>(x=E()&v=0))");
    orR('R=="<{x'=v,v'=a&x<=bf()}++{?x=bf();vi:=v;}{x'=v,v'=-vi^2/(2*(E()-bf()))&x>=bf()}>(x=E()&v=0)|<{x'=v,v'=a&x<=bf()}++{?x=bf();vi:=v;}{x'=v,v'=-vi^2/(2*(E()-bf()))&x>=bf()}>(<{x'=v,v'=a&x<=bf()}++{?x=bf();vi:=v;}{x'=v,v'=-vi^2/(2*(E()-bf()))&x>=bf()}>(x=E()&v=0)|<{x'=v,v'=a&x<=bf()}++{?x=bf();vi:=v;}{x'=v,v'=-vi^2/(2*(E()-bf()))&x>=bf()}><{x'=v,v'=a&x<=bf()}++{?x=bf();vi:=v;}{x'=v,v'=-vi^2/(2*(E()-bf()))&x>=bf()}><{{x'=v,v'=a&x<=bf()}++{?x=bf();vi:=v;}{x'=v,v'=-vi^2/(2*(E()-bf()))&x>=bf()}}*>(x=E()&v=0))");
    diamondOr('R=="<{x'=v,v'=a&x<=bf()}++{?x=bf();vi:=v;}{x'=v,v'=-vi^2/(2*(E()-bf()))&x>=bf()}>(<{x'=v,v'=a&x<=bf()}++{?x=bf();vi:=v;}{x'=v,v'=-vi^2/(2*(E()-bf()))&x>=bf()}>(x=E()&v=0)|<{x'=v,v'=a&x<=bf()}++{?x=bf();vi:=v;}{x'=v,v'=-vi^2/(2*(E()-bf()))&x>=bf()}><{x'=v,v'=a&x<=bf()}++{?x=bf();vi:=v;}{x'=v,v'=-vi^2/(2*(E()-bf()))&x>=bf()}><{{x'=v,v'=a&x<=bf()}++{?x=bf();vi:=v;}{x'=v,v'=-vi^2/(2*(E()-bf()))&x>=bf()}}*>(x=E()&v=0))");
    hideR('R=="x=E()&v=0");
    hideR('R=="<{x'=v,v'=a&x<=bf()}++{?x=bf();vi:=v;}{x'=v,v'=-vi^2/(2*(E()-bf()))&x>=bf()}>(x=E()&v=0)");
    orR('R=="<{x'=v,v'=a&x<=bf()}++{?x=bf();vi:=v;}{x'=v,v'=-vi^2/(2*(E()-bf()))&x>=bf()}><{x'=v,v'=a&x<=bf()}++{?x=bf();vi:=v;}{x'=v,v'=-vi^2/(2*(E()-bf()))&x>=bf()}>(x=E()&v=0)|<{x'=v,v'=a&x<=bf()}++{?x=bf();vi:=v;}{x'=v,v'=-vi^2/(2*(E()-bf()))&x>=bf()}><{x'=v,v'=a&x<=bf()}++{?x=bf();vi:=v;}{x'=v,v'=-vi^2/(2*(E()-bf()))&x>=bf()}><{x'=v,v'=a&x<=bf()}++{?x=bf();vi:=v;}{x'=v,v'=-vi^2/(2*(E()-bf()))&x>=bf()}><{{x'=v,v'=a&x<=bf()}++{?x=bf();vi:=v;}{x'=v,v'=-vi^2/(2*(E()-bf()))&x>=bf()}}*>(x=E()&v=0)");
    hideR('R=="<{x'=v,v'=a&x<=bf()}++{?x=bf();vi:=v;}{x'=v,v'=-vi^2/(2*(E()-bf()))&x>=bf()}><{x'=v,v'=a&x<=bf()}++{?x=bf();vi:=v;}{x'=v,v'=-vi^2/(2*(E()-bf()))&x>=bf()}><{x'=v,v'=a&x<=bf()}++{?x=bf();vi:=v;}{x'=v,v'=-vi^2/(2*(E()-bf()))&x>=bf()}><{{x'=v,v'=a&x<=bf()}++{?x=bf();vi:=v;}{x'=v,v'=-vi^2/(2*(E()-bf()))&x>=bf()}}*>(x=E()&v=0)");
    choiced('R=="<{x'=v,v'=a&x<=bf()}++{?x=bf();vi:=v;}{x'=v,v'=-vi^2/(2*(E()-bf()))&x>=bf()}><{x'=v,v'=a&x<=bf()}++{?x=bf();vi:=v;}{x'=v,v'=-vi^2/(2*(E()-bf()))&x>=bf()}>(x=E()&v=0)");
    choiced('R=="<{x'=v,v'=a&x<=bf()}><{x'=v,v'=a&x<=bf()}++{?x=bf();vi:=v;}{x'=v,v'=-vi^2/(2*(E()-bf()))&x>=bf()}>(x=E()&v=0)|<{?x=bf();vi:=v;}{x'=v,v'=-vi^2/(2*(E()-bf()))&x>=bf()}>#<{x'=v,v'=a&x<=bf()}++{?x=bf();vi:=v;}{x'=v,v'=-vi^2/(2*(E()-bf()))&x>=bf()}>(x=E()&v=0)#");
    orR('R=="<{x'=v,v'=a&x<=bf()}><{x'=v,v'=a&x<=bf()}++{?x=bf();vi:=v;}{x'=v,v'=-vi^2/(2*(E()-bf()))&x>=bf()}>(x=E()&v=0)|<{?x=bf();vi:=v;}{x'=v,v'=-vi^2/(2*(E()-bf()))&x>=bf()}>(<{x'=v,v'=a&x<=bf()}>(x=E()&v=0)|<{?x=bf();vi:=v;}{x'=v,v'=-vi^2/(2*(E()-bf()))&x>=bf()}>(x=E()&v=0))");
    composed('R=="<{?x=bf();vi:=v;}{x'=v,v'=-vi^2/(2*(E()-bf()))&x>=bf()}>(<{x'=v,v'=a&x<=bf()}>(x=E()&v=0)|<{?x=bf();vi:=v;}{x'=v,v'=-vi^2/(2*(E()-bf()))&x>=bf()}>(x=E()&v=0))");
    hideR('R=="<?x=bf();vi:=v;><{x'=v,v'=-vi^2/(2*(E()-bf()))&x>=bf()}>(<{x'=v,v'=a&x<=bf()}>(x=E()&v=0)|<{?x=bf();vi:=v;}{x'=v,v'=-vi^2/(2*(E()-bf()))&x>=bf()}>(x=E()&v=0))");
    choiced('R=="<{x'=v,v'=a&x<=bf()}>#<{x'=v,v'=a&x<=bf()}++{?x=bf();vi:=v;}{x'=v,v'=-vi^2/(2*(E()-bf()))&x>=bf()}>(x=E()&v=0)#");
    solve('R=="<{x'=v,v'=a&x<=bf()}>(<{x'=v,v'=a&x<=bf()}>(x=E()&v=0)|<{?x=bf();vi:=v;}{x'=v,v'=-vi^2/(2*(E()-bf()))&x>=bf()}>(x=E()&v=0))");
    existsR("(sqrt(4*a*bf()-4*a*x_1+v_1^2)-v_1)/2*a", 'R=="\exists t_ (t_>=0&\forall s_ (0<=s_&s_<=t_->a*(s_^2/2)+v_1*s_+x_1<=bf())&\forall v (v=a*t_+v_1->\forall x (x=a*(t_^2/2)+v_1*t_+x_1-><{x'=v,v'=a&x<=bf()}>(x=E()&v=0)|<{?x=bf();vi:=v;}{x'=v,v'=-vi^2/(2*(E()-bf()))&x>=bf()}>(x=E()&v=0))))");
    andR('R=="(sqrt(4*a*bf()-4*a*x_1+v_1^2)-v_1)/2*a>=0&\forall s_ (0<=s_&s_<=(sqrt(4*a*bf()-4*a*x_1+v_1^2)-v_1)/2*a->a*(s_^2/2)+v_1*s_+x_1<=bf())&\forall v (v=a*((sqrt(4*a*bf()-4*a*x_1+v_1^2)-v_1)/2*a)+v_1->\forall x (x=a*(((sqrt(4*a*bf()-4*a*x_1+v_1^2)-v_1)/2*a)^2/2)+v_1*((sqrt(4*a*bf()-4*a*x_1+v_1^2)-v_1)/2*a)+x_1-><{x'=v,v'=a&x<=bf()}>(x=E()&v=0)|<{?x=bf();vi:=v;}{x'=v,v'=-vi^2/(2*(E()-bf()))&x>=bf()}>(x=E()&v=0)))"); <(
      "(sqrt(4*a*bf()-4*a*x_1+v_1^2)-v_1)/2*a>=0":
        todo,
      "\forall s_ (0<=s_&s_<=(sqrt(4*a*bf()-4*a*x_1+v_1^2)-v_1)/2*a->a*(s_^2/2)+v_1*s_+x_1<=bf())&\forall v (v=a*((sqrt(4*a*bf()-4*a*x_1+v_1^2)-v_1)/2*a)+v_1->\forall x (x=a*(((sqrt(4*a*bf()-4*a*x_1+v_1^2)-v_1)/2*a)^2/2)+v_1*((sqrt(4*a*bf()-4*a*x_1+v_1^2)-v_1)/2*a)+x_1-><{x'=v,v'=a&x<=bf()}>(x=E()&v=0)|<{?x=bf();vi:=v;}{x'=v,v'=-vi^2/(2*(E()-bf()))&x>=bf()}>(x=E()&v=0)))":
        todo
    )
    ```

- I had a meeting with Tanner in which we discussed the above proof. We used the
iterateD command in KeYmaera to split up a (*) starred SOMERUNS ODE (Which is
very weak) to its first 4ish runs. We were then able to use diamondOR to
completely remove the starred part of the HP, and were left with a much simpler
proof. Then we used the auto-solve command in KeYmaera to solve the first ODE,
and used the existsR command to instantiate the correct t value to make x equal
to bf to properly set up the rest of the proof. I will now work on moving this
proof to my machine, which I can run KeYmaera on with a better engine (Wolfram
Alpha, not V3), and continue the proof. I will also specify the same proof in
PVS and try to get to the above point. PVS lacks a powerful ODE solving tactic,
so it may be difficult to proceed from there.
- Note: we added `(0 <= a)` to the preconditions of the proof to ensure the
solved t value will not equal 0, since the a is in the numerator.
- After transferring to KeYmeara on my own machine with Wolfram Alpha, I found
some counterexamples. May need to change the preconditions.
- Also need to work on getting PVS set up in WSL on my personal machine. (also
telework permission ?)
- Counter example assumes
  - negative x_1...should that be bf? (-2)
  - negative bf ... this seems alright though if x_1 is also negative (-1)
  - E = 0 ... this seems alright I guess if the others are all negative
  - v_1 and a = 1.0
