<details>
  <summary><b>GOALS</b></summary>
# Goals

- [x] review last journal entry
  - [x] write short summary of last journal entry
  - [x] make progress on last assignment
- [x] complete research abstract
  - [ ] send it to tanner for review

> This journal entry is a clarification of the
> [previous one](2024-02-28.md), written on Feb 28

</details>

## Clarification of Feb 28 journal entry

- $y = T$ is the \[T\]op of the corridor
- $y = 0$ is the bottom of the corridor
- $v_y$ is the max and $-v_y$ is the min velocity in the $y$ direction
- $v_x$ is the constant velocity in the $x$ direction

> The $v_x$ variable is subject to change (see [this journal
> entry](./2024-05-06.md) where I make it not constant)

- $D$ and $-D$ are the maximum and minimum acceleration, respectively
- drone A is approaching drone B, and A is the one we can control.
- We will try to find the largest possible distance drone A needs to be from
  drone B to fully veer to safety and exit the corridor.

To account for the worst possible scenario, assume Drone A is and has reached
its max $y$ velocity while heading towards $y=T$. We can calculate the distance
drone b will travel in the $y$ direction before stopping at $y=T$ with $v_f^2 =
v_0^2 + 2a(\Delta x)$ by making the final $y$ velocity 0.

$v_f^2 = v_0^2 + 2a(\Delta x)$
$$0 ={v_y}^2 + 2 (-D)(T-y)$$
$$-(v_y^2) = -2D(T-y)$$
$$-(v_y^2) = -2DT+2Dy$$
$$2DT-(v_y^2) = 2Dy$$
$$T - \frac{v_y^2}{2D} = y$$

So, to ensure the drone doesn't pass the top of the corridor, it must start
$\frac{v_y^2}{2D}$ away from $y = T$ (the top of the corridor).

---

Lets assume that once the drone reaches $y = T$, it will be at y velocity 0, and
as it begins its descent it will start accelerating towards $y = 0$. The
velocity in the x direction will remain constant.

Now, we can use this information to determine the time it will take for the
drone to reach the same distance from $y = T$ on the other side of the parabola
it is forming with $\Delta y = v_0t + \frac{1}{2}a(t^2)$. Let's substitute known
values:

$$0 = v_yt + \frac{1}{2}(-D)(t^2)$$

And apply the quadratic equation to find the two roots:

> The time variable could also have just been factored out for an easier
> procedure

$$
a = \frac{-D}{2}
\qquad
b = v_y
\qquad
c = 0
\qquad
t = \frac{-b \pm \sqrt{b^2-4ac}}{2a}
$$

$$t = \frac{-v_y \pm \sqrt{v_y^2-4(\frac{-D}{2})(0)}}{-D} $$
$$t = \frac{-v_y \pm \sqrt{v_y^2}}{-D} $$
$$t = \frac{-v_y \pm v_y}{D} $$

We end up with the following roots. The second is the time it will take for the
drone to complete the parabola.

$$
t = 0
\qquad
t = \frac{2v_y}{D}
$$

Since we know how long it will take for the drone to complete the parabola, we
can now calculate how far it will have traveled in the x direction with the
following equation:

> It is important to note that we are assuming constant velocity in the x
> direction here... (fixed in [this journal entry](./2024-05-06.md))

$$\Delta x =v_x(t)$$
$$\Delta x = v_x (\frac{2v_y}{D})$$

Since the drone began its parabola at max y velocity, $v_y$, we can safely assume
that at an identical $y$ location on the opposite side of the parabola the drone
has velocity $-v_y$. We can use this to find out how long it will now take to
reach the bottom of the corridor, $y = 0$, and once again calculate the distance
the drone will travel in the x direction.

$$\Delta y = v_y(t)$$
$$y_f - y_0= v_y(t)$$
$$y_f = y_0 + v_y(t)$$
$$0 = (T - \frac{v_y^2}{2D}) - v_y t$$
$$T - \frac{v_y^2}{2D} = v_y t$$
$$t = \frac{T - \frac{v_y^2}{2D}}{v_y}$$
$$\Delta x = v_x(\frac{T}{v_y} - \frac{v_y}{2D})$$

This gives us the time from the end of the parabola to when the drone hits $y=0$
to exit the corridor. After adding the distance the drone traveled in the
original parabola, we can calculate the distance that drone A must be from its
intersection point with drone B so that it has the room it needs to safely exit
the corridor, $\Delta x$:

$$\Delta x = v_x(\frac{T}{v_y} - \frac{v_y}{2D}) + v_x(\frac{2v_y}{D})$$
$$\Delta x = v_x(\frac{T}{v_y} - \frac{v_y}{2D}+\frac{2v_y}{D})$$
$$\Delta x = v_x(\frac{T}{v_y} - \frac{v_y}{2D}+\frac{4v_y}{2D})$$
$$\Delta x = v_x(\frac{T}{v_y} + \frac{3v_y}{2D})$$

## NEXT:

See [the next journal entry](2024-04-17.md)
